fix: replace Array.Perm and Vector.Perm with one field structures

src/Init/Data/Vector/Perm.lean
@@ -20,13 +20,23 @@ open List Array
 This is a wrapper around `List.Perm`, and for now has much less API.
 For more complicated verification, use `perm_iff_toList_perm` and the `List` API.
 -/
-def Perm (as bs : Vector α n) : Prop :=
-  as.toArray ~ bs.toArray
+structure Perm (as bs : Vector α n) : Prop where
+  of_toArray_perm ::
+  toArray_perm : as.toArray ~ bs.toArray
 
 @[inherit_doc] scoped infixl:50 " ~ " => Perm
 
-theorem perm_iff_toList_perm {as bs : Vector α n} : as ~ bs ↔ as.toList ~ bs.toList := Iff.rfl
-theorem perm_iff_toArray_perm {as bs : Vector α n} : as ~ bs ↔ as.toArray ~ bs.toArray := Iff.rfl
+theorem perm_iff_toArray_perm {as bs : Vector α n} : as ~ bs ↔ as.toArray ~ bs.toArray :=
+  ⟨Perm.toArray_perm, Perm.of_toArray_perm⟩
+
+theorem perm_iff_toList_perm {as bs : Vector α n} : as ~ bs ↔ as.toList ~ bs.toList :=
+  perm_iff_toArray_perm.trans Array.perm_iff_toList_perm
+
+theorem Perm.of_toList_perm {as bs : Vector α n} : as.toList ~ bs.toList → as ~ bs :=
+  perm_iff_toList_perm.mpr
+
+theorem Perm.toList_perm {as bs : Vector α n} : as ~ bs → as.toList ~ bs.toList :=
+  perm_iff_toList_perm.mp
 
 @[simp] theorem perm_mk (as bs : Array α) (ha : as.size = n) (hb : bs.size = n) :
     mk as ha ~ mk bs hb ↔ as ~ bs := by
@@ -35,25 +45,26 @@ theorem perm_iff_toArray_perm {as bs : Vector α n} : as ~ bs ↔ as.toArray ~ b
 theorem toArray_perm_iff (xs : Vector α n) (ys : Array α) : xs.toArray ~ ys ↔ ∃ h, xs ~ Vector.mk ys h := by
   constructor
   · intro h
-    refine ⟨by simp [← h.length_eq], h⟩
+    refine ⟨by simp [← h.size_eq], .of_toArray_perm h⟩
   · intro ⟨h, p⟩
-    exact p
+    exact p.toArray_perm
 
 theorem perm_toArray_iff (xs : Array α) (ys : Vector α n) : xs ~ ys.toArray ↔ ∃ h, Vector.mk xs h ~ ys := by
   constructor
   · intro h
-    refine ⟨by simp [h.length_eq], h⟩
+    refine ⟨by simp [h.size_eq], .of_toArray_perm h⟩
   · intro ⟨h, p⟩
-    exact p
+    exact p.toArray_perm
 
 @[simp, refl] protected theorem Perm.refl (xs : Vector α n) : xs ~ xs := by
   cases xs
   simp
 
-protected theorem Perm.rfl {xs : List α} : xs ~ xs := .refl _
+protected theorem Perm.rfl {xs : Vector α n} : xs ~ xs := .refl _
 
 theorem Perm.of_eq {xs ys : Vector α n} (h : xs = ys) : xs ~ ys := h ▸ .rfl
 
+@[symm]
 protected theorem Perm.symm {xs ys : Vector α n} (h : xs ~ ys) : ys ~ xs := by
   cases xs; cases ys
   simp only [perm_mk] at h
@@ -75,13 +86,24 @@ theorem Perm.mem_iff {a : α} {xs ys : Vector α n} (p : xs ~ ys) : a ∈ xs ↔
   simp at p
   simpa using p.mem_iff
 
-theorem Perm.push (x y : α) {xs ys : Vector α n} (p : xs ~ ys) :
+theorem Perm.append {xs ys : Vector α m} {as bs : Vector α n}
+    (p₁ : xs ~ ys) (p₂ : as ~ bs) : xs ++ as ~ ys ++ bs := by
+  cases xs; cases ys; cases as; cases bs
+  simp only [perm_mk, mk_append_mk] at p₁ p₂ ⊢
+  exact p₁.append p₂
+
+theorem Perm.push (x : α) {xs ys : Vector α n} (p : xs ~ ys) :
+    xs.push x ~ ys.push x := by
+  cases xs; cases ys
+  simp only [perm_mk, push_mk] at p ⊢
+  exact p.push x
+
+theorem Perm.push_comm (x y : α) {xs ys : Vector α n} (p : xs ~ ys) :
     (xs.push x).push y ~ (ys.push y).push x := by
   rcases xs with ⟨xs, rfl⟩
   rcases ys with ⟨ys, h⟩
-  simp only [perm_mk] at p
-  simp only [push_mk, List.append_assoc, singleton_append, perm_toArray]
-  simpa using Array.Perm.push x y p
+  simp only [perm_mk, push_mk] at p ⊢
+  simpa using p.push_comm x y
 
 theorem swap_perm {xs : Vector α n} {i j : Nat} (h₁ : i < n) (h₂ : j < n) :
     xs.swap i j ~ xs := by
@@ -94,10 +116,10 @@ namespace Perm
 set_option linter.indexVariables false in
 theorem extract {xs ys : Vector α n} (h : xs ~ ys) {lo hi : Nat}
     (wlo : ∀ i, i < lo → xs[i]? = ys[i]?) (whi : ∀ i, hi ≤ i → xs[i]? = ys[i]?) :
-    (xs.extract lo hi) ~ (ys.extract lo hi) := by
+    xs.extract lo hi ~ ys.extract lo hi := by
   rcases xs with ⟨xs, rfl⟩
   rcases ys with ⟨ys, h⟩
-  exact Array.Perm.extract h (by simpa using wlo) (by simpa using whi)
+  exact ⟨Array.Perm.extract h.toArray_perm (by simpa using wlo) (by simpa using whi)⟩
 
 end Perm
 
